change CBOR types to fit a common Steel+Pulse+C+Rust subset
following tahina-pro/quackyducky@c03c0d7f6edd06229531317eb42dd4d3d5290aa6

pulse/share/steel/examples/pulse/dice/cbor/CBOR.Pulse.Extern.fsti
@@ -11,6 +11,37 @@ module R = Pulse.Lib.Reference
 module A = Pulse.Lib.Array
 module SM = Pulse.Lib.SeqMatch
 
+val dummy_cbor : cbor
+
+val cbor_map_entry_key: cbor_map_entry -> cbor
+
+val cbor_map_entry_value: cbor_map_entry -> cbor
+
+val cbor_map_entry_key_value_inj
+  (m1 m2: cbor_map_entry)
+: Lemma
+  (requires (
+    cbor_map_entry_key m1 == cbor_map_entry_key m2 /\
+    cbor_map_entry_value m1 == cbor_map_entry_value m2
+  ))
+  (ensures (m1 == m2))
+  [SMTPatOr [
+    [SMTPat (cbor_map_entry_key m1); SMTPat (cbor_map_entry_key m2)];
+    [SMTPat (cbor_map_entry_key m1); SMTPat (cbor_map_entry_value m2)];
+    [SMTPat (cbor_map_entry_value m1); SMTPat (cbor_map_entry_key m2)];
+    [SMTPat (cbor_map_entry_value m1); SMTPat (cbor_map_entry_value m2)];
+  ]]
+
+val mk_cbor_map_entry
+  (key: cbor)
+  (value: cbor)
+: Pure cbor_map_entry
+  (requires True)
+  (ensures (fun res ->
+    cbor_map_entry_key res == key /\
+    cbor_map_entry_value res == value
+  ))
+
 (* Relating a CBOR C object with a CBOR high-level value *)
 
 noextract
@@ -52,22 +83,17 @@ let raw_data_item_map_match
 
 [@@no_auto_projectors]
 noeq
-type read_cbor_success_t = {
+type read_cbor_t = {
+  read_cbor_is_success: bool;
   read_cbor_payload: cbor;
   read_cbor_remainder: A.array U8.t;
   read_cbor_remainder_length: SZ.t;
 }
 
-[@@no_auto_projectors]
-noeq
-type read_cbor_t =
-| ParseError
-| ParseSuccess of read_cbor_success_t
-
 noextract
 let read_cbor_success_postcond
   (va: Ghost.erased (Seq.seq U8.t))
-  (c: read_cbor_success_t)
+  (c: read_cbor_t)
   (v: Cbor.raw_data_item)
   (rem: Seq.seq U8.t)
 : Tot prop
@@ -78,7 +104,7 @@ let read_cbor_success_post
   (a: A.array U8.t)
   (p: perm)
   (va: Ghost.erased (Seq.seq U8.t))
-  (c: read_cbor_success_t)
+  (c: read_cbor_t)
 : Tot vprop
 = exists_ (fun v -> exists_ (fun rem ->
     raw_data_item_match full_perm c.read_cbor_payload v **
@@ -107,9 +133,9 @@ let read_cbor_post
   (va: Ghost.erased (Seq.seq U8.t))
   (res: read_cbor_t)
 : Tot vprop
-= match res with
-  | ParseError -> read_cbor_error_post a p va
-  | ParseSuccess c -> read_cbor_success_post a p va c
+= if res.read_cbor_is_success
+  then read_cbor_success_post a p va res
+  else read_cbor_error_post a p va
 
 val read_cbor
   (a: A.array U8.t)
@@ -125,7 +151,7 @@ val read_cbor
 noextract
 let read_deterministically_encoded_cbor_success_postcond
   (va: Ghost.erased (Seq.seq U8.t))
-  (c: read_cbor_success_t)
+  (c: read_cbor_t)
   (v: Cbor.raw_data_item)
   (rem: Seq.seq U8.t)
 : Tot prop
@@ -136,7 +162,7 @@ let read_deterministically_encoded_cbor_success_post
   (a: A.array U8.t)
   (p: perm)
   (va: Ghost.erased (Seq.seq U8.t))
-  (c: read_cbor_success_t)
+  (c: read_cbor_t)
 : Tot vprop
 = exists_ (fun v -> exists_ (fun rem ->
     raw_data_item_match full_perm c.read_cbor_payload v **
@@ -165,9 +191,9 @@ let read_deterministically_encoded_cbor_post
   (va: Ghost.erased (Seq.seq U8.t))
   (res: read_cbor_t)
 : Tot vprop
-= match res with
-  | ParseError -> read_deterministically_encoded_cbor_error_post a p va
-  | ParseSuccess c -> read_deterministically_encoded_cbor_success_post a p va c
+= if res.read_cbor_is_success
+  then read_deterministically_encoded_cbor_success_post a p va res
+  else read_deterministically_encoded_cbor_error_post a p va
 
 val read_deterministically_encoded_cbor
   (a: A.array U8.t)
