pulse/share/steel/examples/pulse/dice/cbor/CBOR.Pulse.Type.fsti
@@ -28,45 +28,6 @@ val cbor_map_entry: Type0
 
 val cbor: Type0
 
-inline_for_extraction
-noextract
-val dummy_cbor : cbor
-
-inline_for_extraction
-noextract
-val cbor_map_entry_key: cbor_map_entry -> cbor
-
-inline_for_extraction
-noextract
-val cbor_map_entry_value: cbor_map_entry -> cbor
-
-val cbor_map_entry_key_value_inj
-  (m1 m2: cbor_map_entry)
-: Lemma
-  (requires (
-    cbor_map_entry_key m1 == cbor_map_entry_key m2 /\
-    cbor_map_entry_value m1 == cbor_map_entry_value m2
-  ))
-  (ensures (m1 == m2))
-  [SMTPatOr [
-    [SMTPat (cbor_map_entry_key m1); SMTPat (cbor_map_entry_key m2)];
-    [SMTPat (cbor_map_entry_key m1); SMTPat (cbor_map_entry_value m2)];
-    [SMTPat (cbor_map_entry_value m1); SMTPat (cbor_map_entry_key m2)];
-    [SMTPat (cbor_map_entry_value m1); SMTPat (cbor_map_entry_value m2)];
-  ]]
-
-inline_for_extraction
-noextract
-val mk_cbor_map_entry
-  (key: cbor)
-  (value: cbor)
-: Pure cbor_map_entry
-  (requires True)
-  (ensures (fun res ->
-    cbor_map_entry_key res == key /\
-    cbor_map_entry_value res == value
-  ))
-
 val cbor_array_iterator_t: Type0
 
 val cbor_map_iterator_t: Type0
